Define good_dimindex in timeProps

pancake/semantics/timePropsScript.sml
@@ -13,6 +13,12 @@ val _ = set_grammar_ancestry
          "pan_commonProps"];
 
 
+
+Definition good_dimindex_def:
+  good_dimindex (:'a) ⇔
+    dimindex (:'a) = 32 ∨ dimindex (:'a) = 64
+End
+
 Theorem eval_term_inpput_ios_same:
   ∀s m n cnds tclks dest wt s'.
     evalTerm s (SOME m) (Tm (Input n) cnds tclks dest wt) s' ⇒
